skeleton

src/Distributions/UniformPowerOfTwo/Model.dfy
@@ -11,19 +11,23 @@ module UniformPowerOfTwo.Model {
   import Independence
   import Loops
 
-  function UnifStepHelper(m: nat): bool -> Monad.Hurd<nat> {
+  function UnifStepHelper(m: nat): (f: bool -> Monad.Hurd<nat>)
+    ensures forall b :: Monad.IsAlwaysConverging(f(b))
+  {
     (b: bool) => Monad.Return(if b then 2*m + 1 else 2*m)
   }
 
-  function UnifStep(m: nat): Monad.Hurd<nat> {
-    Monad.Bind(Monad.Coin, UnifStepHelper(m))
+  function UnifStep(m: nat): (f: Monad.Hurd<nat>)
+    ensures Monad.IsAlwaysConverging(f)
+  {
+    Monad.Bind(Monad.Coin(), UnifStepHelper(m))
   }
 
   // Adapted from Definition 48 (see issue #79 for the reason of the modification)
   // The return value u is uniformly distributed between 0 <= u < 2^k where 2^k <= n < 2^(k + 1).
   opaque function Sample(n: nat): (h: Monad.Hurd<nat>)
     requires n >= 1
-    ensures forall s :: Sample(n)(s).Result? // always terminates, not just almost surely
+    ensures Monad.IsAlwaysConverging(h) // always terminates, not just almost surely
   {
     if n == 1 then
       Monad.Return(0)
@@ -31,120 +35,4 @@ module UniformPowerOfTwo.Model {
       Monad.Bind(Sample(n/2), UnifStep)
   }
 
-  // A tail recursive version of Sample, closer to the imperative implementation
-  function SampleTailRecursive(n: nat, u: nat := 0): Monad.Hurd<nat>
-    requires n >= 1
-  {
-    (s: Rand.Bitstream) =>
-      if n == 1 then
-        Monad.Result(u, s)
-      else
-        SampleTailRecursive(n / 2, if Rand.Head(s) then 2*u + 1 else 2*u)(Rand.Tail(s))
-  }
-
-  // Equivalence of Sample and its tail-recursive version
-  lemma SampleCorrespondence(n: nat, s: Rand.Bitstream)
-    requires n >= 1
-    ensures SampleTailRecursive(n)(s) == Sample(n)(s)
-  {
-    if n == 1 {
-      reveal Sample();
-      assert SampleTailRecursive(n)(s) == Sample(n)(s);
-    } else {
-      var k := Helper.Log2Floor(n);
-      assert Helper.Power(2, k) <= n < Helper.Power(2, k + 1) by { Helper.Power2OfLog2Floor(n); }
-      calc {
-        SampleTailRecursive(n)(s);
-        { SampleTailRecursiveEqualIfSameLog2Floor(n, Helper.Power(2, k), k, 0, s); }
-        SampleTailRecursive(Helper.Power(2, k))(s);
-        Monad.Bind(Sample(Helper.Power(2, 0)), (u: nat) => SampleTailRecursive(Helper.Power(2, k), u))(s);
-        { RelateWithTailRecursive(k, 0, s); }
-        Sample(Helper.Power(2, k))(s);
-        { SampleEqualIfSameLog2Floor(n, Helper.Power(2, k), k, s); }
-        Sample(n)(s);
-      }
-    }
-  }
-
-  // All numbers between consecutive powers of 2 behave the same as arguments to SampleTailRecursive
-  lemma SampleTailRecursiveEqualIfSameLog2Floor(m: nat, n: nat, k: nat, u: nat, s: Rand.Bitstream)
-    requires m >= 1
-    requires n >= 1
-    requires Helper.Power(2, k) <= m < Helper.Power(2, k + 1)
-    requires Helper.Power(2, k) <= n < Helper.Power(2, k + 1)
-    ensures SampleTailRecursive(m, u)(s) == SampleTailRecursive(n, u)(s)
-  {
-    if k == 0 {
-      assert m == n;
-    } else {
-      assert 1 <= m;
-      assert 1 <= n;
-      calc {
-        SampleTailRecursive(m, u)(s);
-        SampleTailRecursive(m / 2, if Rand.Head(s) then 2*u + 1 else 2*u)(Rand.Tail(s));
-        { SampleTailRecursiveEqualIfSameLog2Floor(m / 2, n / 2, k - 1, if Rand.Head(s) then 2*u + 1 else 2*u, Rand.Tail(s)); }
-        SampleTailRecursive(n / 2, if Rand.Head(s) then 2*u + 1 else 2*u)(Rand.Tail(s));
-        SampleTailRecursive(n, u)(s);
-      }
-    }
-  }
-
-  // All numbers between consecutive powers of 2 behave the same as arguments to Sample
-  lemma SampleEqualIfSameLog2Floor(m: nat, n: nat, k: nat, s: Rand.Bitstream)
-    requires m >= 1
-    requires n >= 1
-    requires Helper.Power(2, k) <= m < Helper.Power(2, k + 1)
-    requires Helper.Power(2, k) <= n < Helper.Power(2, k + 1)
-    ensures Sample(m)(s) == Sample(n)(s)
-  {
-    if k == 0 {
-      assert m == n;
-    } else {
-      assert 1 <= m;
-      assert 1 <= n;
-      calc {
-        Sample(m)(s);
-        { reveal Sample(); }
-        Monad.Bind(Sample(m / 2), UnifStep)(s);
-        { SampleEqualIfSameLog2Floor(m / 2, n / 2, k - 1, s); }
-        Monad.Bind(Sample(n / 2), UnifStep)(s);
-        { reveal Sample(); }
-        Sample(n)(s);
-      }
-    }
-  }
-
-  // The induction invariant for the equivalence proof (generalized version of SampleCorrespondence)
-  lemma RelateWithTailRecursive(l: nat, m: nat, s: Rand.Bitstream)
-    decreases l
-    ensures Monad.Bind(Sample(Helper.Power(2, m)), (u: nat) => SampleTailRecursive(Helper.Power(2, l), u))(s) == Sample(Helper.Power(2, m + l))(s)
-  {
-    if l == 0 {
-      calc {
-        Monad.Bind(Sample(Helper.Power(2, m)), (u: nat) => SampleTailRecursive(Helper.Power(2, l), u))(s);
-        (var Result(u, s') := Sample(Helper.Power(2, m))(s); SampleTailRecursive(1, u)(s'));
-        Sample(Helper.Power(2, m + l))(s);
-      }
-    } else {
-      assert LGreaterZero: Helper.Power(2, l) >= 1 by { Helper.PowerGreater0(2, l); }
-      assert MGreaterZero: Helper.Power(2, m) >= 1 by { Helper.PowerGreater0(2, m); }
-      assert L1GreaterZero: Helper.Power(2, l - 1) >= 1 by { Helper.PowerGreater0(2, l - 1); }
-      calc {
-        Monad.Bind(Sample(Helper.Power(2, m)), (u: nat) => SampleTailRecursive(Helper.Power(2, l), u))(s);
-        (var Result(u, s') := Sample(Helper.Power(2, m))(s); SampleTailRecursive(Helper.Power(2, l), u)(s'));
-        { reveal LGreaterZero; }
-        (var Result(u, s') := Sample(Helper.Power(2, m))(s);
-         SampleTailRecursive(Helper.Power(2, l) / 2, if Rand.Head(s') then 2 * u + 1 else 2 * u)(Rand.Tail(s')));
-        { assert Helper.Power(2, l) / 2 == Helper.Power(2, l - 1); reveal L1GreaterZero; }
-        (var Result(u', s') := Monad.Bind(Sample(Helper.Power(2, m)), UnifStep)(s);
-         SampleTailRecursive(Helper.Power(2, l - 1), u')(s'));
-        { assert Helper.Power(2, m + 1) / 2 == Helper.Power(2, m); reveal Sample(); }
-        (var Result(u', s') := Sample(Helper.Power(2, m + 1))(s);
-         SampleTailRecursive(Helper.Power(2, l - 1), u')(s'));
-        Monad.Bind(Sample(Helper.Power(2, m + 1)), (u: nat) => SampleTailRecursive(Helper.Power(2, l - 1), u))(s);
-        { RelateWithTailRecursive(l - 1, m + 1, s); }
-        Sample(Helper.Power(2, m + l))(s);
-      }
-    }
-  }
 }
